interpreter/InterpreterTest/Ast.lean
@@ -1,0 +1,5 @@
+inductive Ast : Type where
+  | val : Int → Ast
+  | var : String → Ast
+  | add : Ast → Ast → Ast
+  | let_ : String → Ast → Ast → Ast
