interpreter/InterpreterTest/Parse.lean
@@ -1,0 +1,178 @@
+import InterpreterTest.Ast
+
+abbrev ParseInput := List Char
+
+inductive Error : Type where
+  deriving Repr
+
+/--
+An optional value α, with additional errors emitted and where
+the rest of the input.
+-/
+structure ParseResult (α : Type) : Type where
+  value : Option α
+  rest : ParseInput
+  errors : List Error
+  errorsNotNil : value = none → errors ≠ []
+  deriving Repr
+
+@[simp] def Parser ret := ParseInput → ParseResult ret
+
+namespace ParseResult
+
+  -- Simple ways to construct
+
+  def success (value : α) (rest : ParseInput) : ParseResult α :=
+    { value := some value
+      rest := rest
+      errors := []
+      errorsNotNil := by simp }
+
+  def fromErrors (errors : List Error) (rest : ParseInput) (h : errors ≠ [])
+  : ParseResult α :=
+    { value := none
+      rest := rest
+      errors := errors
+      errorsNotNil := fun _ => h }
+
+  abbrev fromError (error : Error) (rest : ParseInput) : ParseResult α :=
+    fromErrors [error] rest (by simp)
+
+  -- Properties
+
+  def isSuccess (self : ParseResult α) : Bool := self.value.isSome
+
+  @[simp]
+  theorem isSuccess_success {α value rest}
+  : isSuccess (@success α value rest) = true := by
+    unfold success isSuccess
+    cases h : success value rest
+    simp_all
+
+  theorem isSuccess_fromErrors {α errors rest h}
+  : isSuccess (@fromErrors α errors rest h) = false := by
+    unfold fromErrors isSuccess
+    cases h : (fromErrors errors rest h : ParseResult α)
+    simp_all
+
+  @[simp]
+  theorem errors_eq_nil : errors result = [] → result.isSuccess = true := by
+    by_contra
+    simp
+
+  theorem not_success (h : !isSuccess self) : self.value.isNone :=
+    by simp at h; simp_all
+
+  def map : ParseResult a -> (a -> b) -> ParseResult b
+    | { value := none, errors := e, rest := r, .. }, _ =>
+      fromErrors e r (by simp_all)
+    | { value := some value, rest := rest, .. }, f => success (f value) rest
+
+  theorem map_not_isSuccess
+  (self : ParseResult a) (f : a -> b) (h : isSuccess self = false)
+  : (self.map f).isSuccess = false := by
+    rcases self
+    simp_all [map]
+
+  theorem map_isSuccess_eq_success
+  (self : ParseResult a) (f : a -> b) (h : isSuccess self)
+  : self.map f = success (f <| self.value.get (by simp_all)) self.rest := by
+    rcases self with ⟨value⟩
+    unfold map
+    unfold isSuccess at h
+    simp at h
+    cases value
+    . contradiction
+    . simp_all
+
+  theorem map_isSuccess
+  (self : ParseResult a) (f : a -> b) (h : isSuccess self)
+  : (self.map f).isSuccess := by simp_all
+
+  def andThen (self : ParseResult α) (f : (α × ParseInput) → ParseResult β)
+  : ParseResult β :=
+    match h : self.value with
+    | some value =>
+      let next := f (value, self.rest)
+      let allErrors := self.errors ++ next.errors
+      have : next.value.isNone → allErrors ≠ [] := fun _ =>
+        have : next.errors ≠ [] := by simp_all
+        by simp [this, allErrors]
+      { value := next.value
+        rest := next.rest
+        errors := allErrors
+        errorsNotNil := by assumption
+      }
+    | none =>
+      have : self.errors ≠ [] := by simp_all
+      fromErrors self.errors self.rest (h := this)
+      
+  theorem andThen_not_isSuccess
+  (self: ParseResult α)
+  (notSuccess : self.isSuccess = false)
+  (f : (α × ParseInput) → ParseResult β)
+  : (self.andThen f).isSuccess = false := by
+    rcases self with ⟨value⟩
+    have : value = none := by simp_all
+    subst this
+    unfold andThen
+    simp
+      
+  theorem andThen_isSuccess
+  (self: ParseResult α)
+  (notSuccess : self.isSuccess)
+  (f : (α × ParseInput) → ParseResult β)
+  : (self.andThen f).isSuccess = (f (self.value.get (by simp_all), self.rest)).isSuccess := by
+    rcases self with ⟨value⟩
+    cases value
+    . exact Bool.noConfusion notSuccess
+    . unfold andThen
+      simp_all
+
+end ParseResult
+
+namespace Parser
+
+  def success (val : α) : Parser α :=
+    fun input => ParseResult.success val input
+
+  def fromError (error : Error) : Parser α :=
+    fun input => ParseResult.fromError error input
+
+  abbrev run (parser : Parser α) (input : ParseInput) : ParseResult α :=
+    parser input
+
+  def andThen (first : Parser a) (second : a -> Parser b) : Parser b :=
+    fun input =>
+      let firstResult := first input
+      firstResult.andThen fun (value, rest) => second value rest
+      
+  theorem andThen_isSuccess
+  (first : Parser a) (second : a -> Parser b) (input : ParseInput)
+  (h : first.run input |>.isSuccess)
+  : ((first.andThen second).run input).isSuccess = (second (first.run input |>.value.get (by simp_all)).value input).isSome := by
+    simp_all
+
+end Parser
+
+def parse_sequence (condition : Char → Option α)
+: Parser (List α) := fun input =>
+  match input with
+  | [] => ParseResult.success [] []
+  | c :: cs =>
+    if let Option.some x := condition c then
+      cs |> Parser.run (
+        Parser.success x |>.andThen fun x =>
+        parse_sequence condition
+      )
+    else
+      ParseResult.failure
+
+def parse_literal (str : String) : ParseResult Ast := by
+  sorry
+
+example : parse_literal "42" = some (Ast.val 42) := by
+  sorry
+
+def parse (str : String) : Option Ast := sorry
+  
